store/client_proofs/create.v
@@ -35,47 +35,26 @@ Lemma wp_client_create c kI kR cs t1 t2 :
   {{{ db_connected kI kR cs ∗
       rem_free_at kI kR {[t1]} }}}
     Client.create N c (repr cs) t1 t2
-  {{{ (b : bool), RET #b;
+  {{{ RET #();
       db_connected kI kR cs ∗
       rem_mapsto kI kR t1 t2 }}}.
 Proof.
 iIntros "#chan_c (_ & _ & _ & _ & _ & _ & #create & #ack & _) #p_t1 #p_t2".
 iIntros "!> %Φ [client free] post".
-iDestruct "client" as "(%n & %beginning & client & conn)".
-iPoseProof (client_connected_wf_conn_state with "conn") as "#?".
-rewrite /Client.create. wp_pures.
+iDestruct "client" as "(%n & %beginning & client & conn & token)".
 iMod (@rem_mapsto_alloc _ _ _ _ _ _ t1 t2 with "client free")
   as "(client & mapsto & _ & #created)".
 { by rewrite elem_of_singleton. }
-wp_bind (Connection.timestamp _).
-iApply (wp_connection_timestamp_client with "conn").
-iIntros "!> conn". wp_pures.
-wp_bind (Connection.tick _).
-iApply (wp_connection_tick_client with "conn"). iIntros "!> conn".
-iDestruct (create_predI with "conn p_t1 p_t2 created")
-  as "#p_m1".
-wp_list. wp_bind (tint _). iApply wp_tint. wp_list. wp_term_of_list. wp_pures.
-wp_bind (Connection.send _ _ _ _).
-iApply (wp_connection_send with "[//] create [] []") => //.
-{ by rewrite public_of_list /= public_TInt; eauto. }
-{ by iIntros "!> _". }
-iIntros "!> _". wp_pures.
-iCombine "client mapsto post" as "I". iRevert "conn I".
-iApply wp_connection_recv_client => //.
-iIntros "!> %m conn (client & mapsto & post) #m_m #inv'".
-wp_pures. wp_list_of_term m; wp_pures; last by iLeft; iFrame.
-wp_list_match => [ts' k' v' b -> {m}|_] /=; wp_pures; last by iLeft; iFrame.
-wp_bind (tint _). iApply wp_tint.
-wp_eq_term e; wp_pures; last by iLeft; iFrame.
-subst ts'.
-wp_eq_term e; wp_pures; last by iLeft; iFrame.
-subst k'.
-wp_eq_term e; wp_pures; last by iLeft; iFrame.
-subst v'.
-wp_bind (tint _). iApply wp_tint.
-wp_bind (eq_term _ _). iApply wp_eq_term. wp_pures.
-iRight. iModIntro. iExists _. iSplit => //. iApply "post".
-by iFrame; eauto.
+wp_lam. wp_pures. wp_list.
+wp_apply (wp_connection_write with "[//] [] [] [] [$]") => //.
+- by rewrite /=; eauto.
+- iRight. iExists _, _. by eauto.
+iIntros "conn". wp_pures.
+wp_apply (wp_connection_read with "[//] [] [$]") => //.
+- iIntros "%ts (conn & _ & _)". wp_pures.
+wp_apply (wp_connection_tick with "[$]").
+iIntros "conn". iApply "post".
+by iFrame.
 Qed.
 
 End Verif.
