store/client_proofs/store.v
@@ -27,54 +27,6 @@ Implicit Types v : val.
 
 Variable N : namespace.
 
-Lemma wp_client_send_store c kI kR cs t1 t2 t2' :
-  channel c -∗
-  store_ctx N -∗
-  public t1 -∗
-  public t2' -∗ (* FIXME: t1 and t2' shouldn't have to be public already *)
-  {{{ db_connected kI kR cs ∗ rem_mapsto kI kR t1 t2 }}}
-    Client.send_store N c (repr cs) t1 t2'
-  {{{ RET #(); db_connected kI kR cs ∗ rem_mapsto kI kR t1 t2' }}}.
-Proof.
-iIntros "#chan_c (_ & _ & #? & _) #p_t1 #p_t2' !> %Φ [client mapsto] post".
-iDestruct "client" as "(%n & %beginning & client & conn)".
-iMod (rem_mapsto_store t2' with "client mapsto")
-  as "(client & mapsto & #update)".
-wp_lam. wp_pures.
-wp_apply (wp_connection_timestamp_client with "conn"); iIntros "conn".
-wp_pures. wp_apply (wp_connection_tick_client with "conn"). iIntros "conn".
-iPoseProof (store_predI with "[$] update") as "#?".
-wp_pures. wp_list. wp_bind (tint _). iApply wp_tint. wp_list.
-wp_term_of_list. wp_pures.
-iPoseProof (client_connected_wf_conn_state with "conn") as "#conn'".
-iApply (wp_connection_send with "[//] [//] [] [#] conn'") => //.
-{ rewrite public_of_list /= public_TInt. by eauto. }
-{ by iIntros "!> _". }
-iIntros "!> _".
-iApply "post". by iFrame.
-Qed.
-
-Lemma wp_client_ack_store c kI kR cs :
-  channel c -∗
-  store_ctx N -∗
-  {{{ db_connected kI kR cs }}}
-    Client.ack_store N c (repr cs)
-  {{{ RET #(); db_connected kI kR cs }}}.
-Proof.
-iIntros "#chan_c (_ & _ & _ & #? & _) !> %Φ client post".
-iDestruct "client" as "(%n & %beginning & client & conn)".
-rewrite /Client.ack_store. wp_pures.
-wp_apply (wp_connection_timestamp_client with "conn"). iIntros "conn".
-wp_pures.
-iCombine "client post" as "I". iRevert "conn I".
-iApply wp_connection_recv_client => //.
-iIntros "!> %m conn (client & post) #m_m _".
-wp_pures. wp_apply wp_tint.
-wp_eq_term e; wp_pures; last by iLeft; iFrame.
-iRight. iModIntro. iExists _. iSplit => //.
-iApply "post". by iExists _, _; iFrame; eauto.
-Qed.
-
 Lemma wp_client_store c kI kR cs t1 t2 t2' :
   channel c -∗
   store_ctx N -∗
@@ -85,13 +37,19 @@ Lemma wp_client_store c kI kR cs t1 t2 t2' :
   {{{ RET #(); db_connected kI kR cs ∗ rem_mapsto kI kR t1 t2' }}}.
 Proof.
 iIntros "#chan_c #ctx #p_t1 #p_t2 !> %Φ [client mapsto] post".
-rewrite /Client.store.
-wp_pures. wp_bind (Client.send_store _ _ _ _ _).
-iApply (wp_client_send_store with "[] [] [] [//] [$client $mapsto] [post]")
-  => //.
-iIntros "!> [client mapsto]". wp_pures.
-iApply (wp_client_ack_store with "[] [] [client] [post mapsto]") => //.
-iIntros "!> client". iApply "post". by iFrame.
+iDestruct "client" as "(%n & %n0 & db & conn & token)".
+wp_lam. wp_pures. wp_list.
+iMod (rem_mapsto_store t2' with "db mapsto") as "(db & mapsto & #store)".
+wp_apply (wp_connection_write with "[//] [] [] [] [$]").
+- by iApply store_ctx_store.
+- rewrite /=; eauto.
+- iRight. by iExists t1, t2'; eauto.
+iIntros "conn". wp_pures.
+wp_apply (wp_connection_read with "[//] [] [$]").
+- by iApply store_ctx_ack_store.
+iIntros "%ts [conn _]". wp_pures.
+wp_apply (wp_connection_tick with "[$]"). iIntros "conn".
+iApply "post". by iFrame.
 Qed.
 
 End Verif.
